coq/theories/ITree/ITree.v
@@ -1,22 +1,20 @@
-Set Implicit Arguments.
-Set Contextual Implicit.
-Set Primitive Projections.
-
-From Equations Require Import Equations.
-
 From OGS Require Import Utils.
-From OGS.ITree Require Import Cat Event.
+From OGS.Game Require Import Event.
 
-Section itree. Context {I : Type} {E : event I I} {R : I -> Type}.
 
-  Variant itreeF (ind : I -> Type) (i : I) :=
-  | RetF (r : R i)
-  | TauF (t : ind i)
-  | VisF (e : E.(qry) i) (k : forall r : E.(rsp) e, ind (E.(nxt) e r))
+Section itree.
+  Context {I : Type}.
+  Context (E : event I I).
+  Context (R : psh I).
+
+  Variant itreeF (REC : psh I) (i : I) : Type :=
+    | RetF (r : R i) : itreeF REC i
+    | TauF (t : REC i) : itreeF REC i
+    | VisF (q : E.(e_qry) i) (k : forall (r : E.(e_rsp) q), REC (E.(e_nxt) r)) : itreeF REC i
   .
+  Derive NoConfusion for itreeF.
 
-  CoInductive itree (i : I) : Type := go
-  { _observe : itreeF itree i }.
+  CoInductive itree (i : I) : Type := go { _observe : itreeF itree i }.
 
 End itree.
 
@@ -25,63 +23,16 @@ Bind Scope itree_scope with itree.
 Delimit Scope itree_scope with itree.
 Local Open Scope itree_scope.
 
-Arguments itree {_} _ _ _.
-Arguments itreeF {_} _ _ _ _.
+Arguments itree {I} E R i.
+Arguments itreeF {I} E R REC i.
+Arguments RetF {I E R REC i} r.
+Arguments TauF {I E R REC i} t.
+Arguments VisF {I E R REC i} q k.
 
 Notation itree' E R := (itreeF E R (itree E R)).
 
-Definition observe {I E R i} (t : @itree I E R i) : itree' E R i :=
-  @_observe I E R i t.
+Definition observe {I E R i} (t : @itree I E R i) : itree' E R i := @_observe I E R i t.
 
-Notation Ret x := (go (RetF x)).
-Notation Tau t := (go (TauF t)).
-Notation Vis e k := (go (VisF e k)).
-
-Section short. Context {I} {E : event I I} {R : I -> Type}.
-
-  Definition ret {i} x : itree E R i := Ret x.
-  Definition tau {i} t : itree E R i := Tau t.
-  Definition vis {i} e k : itree E R i := Vis e k.
-  Definition vis_alg : ⟦ E ⟧ (itree E R) ⇒ᵢ itree E R :=
-    fun _ x => Vis (projT1 x) (projT2 x).
-
-End short.
-
-Definition vis' {I} (E : event I I) {R i} e k : itree E R i := @vis _ E _ _ e k.
-Arguments vis' {I} E {R i} e k.
-
-Section structure. Context {I : Type} {E : event I I} {X Y : psh I}.
-
-  Definition fmap (f : X ⇒ᵢ Y) : itree E X ⇒ᵢ itree E Y :=
-    cofix _fmap _ u :=
-      match (observe u) with
-      | RetF r => Ret (f _ r)
-      | TauF t => Tau (_fmap _ t)
-      | VisF e k => vis e (fun r => _fmap _ (k r))
-      end.
-
-  Definition subst (f : X ⇒ᵢ itree E Y) : itree E X ⇒ᵢ itree E Y :=
-    cofix _subst _ u :=
-      match observe u with
-      | RetF r => f _ r
-      | TauF t => Tau (_subst _ t)
-      | VisF e k => Vis e (fun r => _subst _ (k r))
-      end.
-
-  (* McBride's "daemonic" bind: [f] has to be defined at every state [i] *)
-  Definition bind {i} x f := @subst f i x.
-
-End structure.
-(*Notation "x ?>= f" := (bind x f) (at level 20).*)
-
-Instance FunctorItree {I} (E : event I I) : Functor (itree E) :=
-  Build_Functor _ (fun X Y => @fmap I E X Y).
-
-Instance MonadItree {I} (E : event I I) : Monad (itree E) :=
-  Build_Monad _ (fun X => @ret I E X) (fun X Y => @subst I E X Y).
-
-Definition kcomp {I} {E : event I I} {X Y Z : psh I} (f : X ⇒ᵢ itree E Y) (g : Y ⇒ᵢ itree E Z) : X ⇒ᵢ itree E Z :=
-  fun i x => f i x >>= g.
-
-#[global]
-Notation "f >> g" := (kcomp f g) (at level 30).
+Notation Ret' x := (go (RetF x)).
+Notation Tau' t := (go (TauF t)).
+Notation Vis' e k := (go (VisF e k)).
